fix: incorporate code review comments and awesome new info from Leo and Henrik.

SimpleMonads/Monads.lean
@@ -5,23 +5,29 @@ def divide (x: Float ) (y: Float): ExceptT String Id Float :=
   else
     pure (x / y)
 
+#eval divide 5 0  -- Except.error "can't divide by zero"
+
 #check (Except String) -- Type u_1 → Type (max 0 u_1)
 
+#check ExceptT String Id
+
 def test :=
-  for x in [1:10] do
-    for y in [0:10] do
-      discard (divide x.toFloat y.toFloat)
+  divide 5 0
 
-#eval (test).run -- Except.error "can't divide by zero"
+#check test  -- ExceptT String Id Float
 
-#eval test -- interesting, eval doesn't need (test).run in this case.
+#eval test -- Except.error "can't divide by zero"
+
+#eval test.run -- this was done implicitly for us
+
+#eval test |>.run -- this is the best way to call run if run takes arguments.
 
 #check  (Except.pure 6.5) --  Except ?m.727 Float
 
-def testCatch := do
+def testCatch :=
     try
       let r ← divide 8 0
-      return toString r -- ExceptT String Id String
+      return toString r -- 'r' is type Float
     catch e =>
       return s!"Caught exception: {e}"
 
@@ -29,28 +35,57 @@ def testCatch := do
 
 #eval testCatch -- Caught exception: can't divide by zero
 
-#check ExceptT String Id PUnit
+/- unwrap Except using match -/
+def testUnwrap : String := Id.run do
+    let r := divide 8 0 -- r is type ExceptT String Id Float
+    match r with
+    | .ok a => toString a -- 'a' is type Float
+    | .error e => s!"Caught exception: {e}"
 
-#eval divide 5 0  -- Except.error "can't divide by zero"
+#check testUnwrap -- String
+#eval testUnwrap -- "Caught exception: can't divide by zero"
+
+/- unwrap Except using coercion -/
+instance : Coe (ExceptT α Id α) α where
+  coe a := match a with
+    | .ok v => v
+    | .error v => v
+
+def testCoerce : String :=
+  let act : ExceptT String Id String := do
+    let r ← divide 8 0
+    return r.toString
+  act
+
+#check testCoerce -- String
+#eval testCoerce  -- "can't divide by zero"
+
+/- adding StateT -/
 
 def divideLog (x: Float ) (y: Float): StateT Nat Id Float :=
   if y == 0 then
     return 0
   else do
-    (modify) fun s => s + 1
+    modify fun s => s + 1
     return x / y
+
+#check divideLog              -- Float → Float → StateT Nat Id Float
+#reduce StateT Nat Id Float   -- Nat → Float × Nat
+
+#eval divideLog 8 4 0         -- (2.000000, 1)
+#eval (divideLog 8 4).run 0   -- (2.000000, 1)
+#eval divideLog 8 4 |>.run 0  -- (2.000000, 1)
 
 def testDivideLog := do
   let mut state := 0
   for x in [0:10] do
     for y in [0:10] do
-      let r ← (divideLog x.toFloat y.toFloat) state
+      let r ← divideLog x.toFloat y.toFloat |>.run state
       state := r.2
   state
 
 
 #eval testDivideLog -- 90
-
 
 /- chaining monads using bind -/
 def divideIt (x:Float) (y:Float) : StateT Nat (ExceptT String Id) Float :=
@@ -63,14 +98,14 @@ def divideIt (x:Float) (y:Float) : StateT Nat (ExceptT String Id) Float :=
 
 #reduce StateT Nat (ExceptT String Id) Float
 
-#eval divideIt 5 2 0 -- Except.ok (5.000000, 1)
+#eval divideIt 5 2 |>.run 0 -- Except.ok (5.000000, 1)
 
 def testIt := do
   let mut log := 0
   for x in [0:10] do
     for y in [0:10] do
       try
-        let r ← divideIt x.toFloat y.toFloat log
+        let r ← divideIt x.toFloat y.toFloat |>.run log
         log := r.2
       catch _  =>
         pure ()
@@ -86,48 +121,49 @@ def divideDo (x:Float) (y:Float) : (StateT Nat (ExceptT String Id)) Float := do
     modify fun s => s + 1
     pure (x / y)
 
-#eval divideDo 5 2 0 -- Except.ok (2.500000, 1)
+#eval divideDo 5 2 |>.run 0 -- Except.ok (2.500000, 1)
 
-
+/- Adding ReadeT monad -/
 def divideWithArgs (x:Float) (y:Float) : ReaderT (List String) (StateT Nat (ExceptT String Id)) Float :=
-  if y == 0 then
-    throw "can't divide by zero"
-  else
-    bind (modify fun s => s + 1) fun _ =>
-      bind (get) fun s =>
-        bind (read) fun args =>
-          if (s > 10 && args.contains "--limit") then
-            throw "too many divides"
-          else
-            pure (x / y)
+  bind (modify fun s => s + 1) fun _ =>
+    bind (get) fun s =>
+      bind (read) fun args =>
+        if (s > 10 && args.contains "--limit") then
+          throw "too many divides"
+        else if y == 0 then
+          throw "can't divide by zero"
+        else
+          pure (x / y)
 
 /-
 List String → Nat → Except String (Float × Nat)
 -/
 #reduce ReaderT (List String) (StateT Nat (ExceptT String Id)) Float
 
-#eval divideWithArgs 5 2 [] 0 -- Except.ok (2.500000, 1)
-#eval divideWithArgs 5 0 [] 0 -- Except.error "can't divide by zero"
-#eval divideWithArgs 5 2 ["--limit"] 10 -- Except.error "too many divides"
-
+#eval divideWithArgs 5 2 |>.run [] |>.run 0 -- Except.ok (2.500000, 1)
+#eval divideWithArgs 5 0 |>.run [] |>.run 0 -- Except.error "can't divide by zero"
+#eval divideWithArgs 5 2 |>.run ["--limit"] |>.run 10 -- Except.error "too many divides"
 
 def divideWithArgsDo (x:Float) (y:Float) : ReaderT (List String) (StateT Nat (ExceptT String Id)) Float := do
-  if y == 0 then
+  modify fun s => s + 1
+  let s ← get
+  let args ← read
+  if (s > 10 && args.contains "--limit") then
+    throw "too many divides"
+  else if y == 0 then
     throw "can't divide by zero"
   else
-    modify fun s => s + 1
-    let s ← get
-    let args ← read
-    if (s > 10 && args.contains "--limit") then
-      throw "too many divides"
-    else
-      pure (x / y)
+    pure (x / y)
 
-#eval divideWithArgsDo 5 2 [] 0 -- Except.ok (2.500000, 1)
-#eval divideWithArgsDo 5 0 [] 0 -- Except.error "can't divide by zero"
-#eval divideWithArgsDo 5 2 ["--limit"] 10 -- Except.error "too many divides"
+#eval divideWithArgsDo 5 2 |>.run [] |>.run 0 -- Except.ok (2.500000, 1)
+#eval divideWithArgsDo 5 0 |>.run [] |>.run 0 -- Except.error "can't divide by zero"
+#eval divideWithArgsDo 5 2 |>.run ["--limit"] |>.run 10 -- Except.error "too many divides"
 
+/- proof that these are the same-/
+example : divideWithArgs x y = divideWithArgsDo x y := by
+  simp[divideWithArgs, divideWithArgsDo]    -- Goals accomplished 🎉
 
+/- monad composition using lifting -/
 def divideRefactored (x:Float) (y:Float) : ReaderT (List String) (StateT Nat (ExceptT String Id)) Float := do
   modify fun s => s + 1
   let s ← get
@@ -137,7 +173,10 @@ def divideRefactored (x:Float) (y:Float) : ReaderT (List String) (StateT Nat (Ex
   else
     divide x y
 
-#eval divideRefactored 5 0 [] 0 -- Except.error "can't divide by zero"
+
+#eval divideRefactored 5 2 |>.run [] |>.run 0 -- Except.ok (2.500000, 1)
+#eval divideRefactored 5 0 |>.run [] |>.run 0 -- Except.error "can't divide by zero"
+#eval divideRefactored 5 2 |>.run ["--limit"] |>.run 10 -- Except.error "too many divides"
 
 #reduce ReaderT (List String) (StateT Nat (ExceptT String Id)) Float
 #reduce ExceptT String Id Float
@@ -149,7 +188,7 @@ def lift1 (x : ExceptT String Id Float) : (StateT Nat (ExceptT String Id)) Float
 
 #reduce lift1 -- fun x s => Except.rec (fun a => Except.error a) (fun a => Except.ok (a, s)) x
 
-#eval lift1 (divide 5 1) 3 -- Except.ok (5.000000, 3)
+#eval lift1 (divide 5 1) |>.run 3 -- Except.ok (5.000000, 3)
 
 def lift2 (x : StateT Nat (ExceptT String Id) Float)  : ReaderT (List String) (StateT Nat (ExceptT String Id)) Float :=
   x
@@ -159,4 +198,4 @@ def transitive (x : StateT Nat (ExceptT String Id) Float) := do
   lift2 x
 
 
-#eval lift2 (lift1 (divide 5 1)) ["discarded", "state"] 0 -- Except.ok (5.000000, 0)
+#eval lift2 (lift1 (divide 5 1)) |>.run ["discarded", "state"] |>.run 4 -- Except.ok (5.000000, 4)
