SimpleMonads/Main.lean
@@ -1,13 +1,18 @@
 import Monads
 
-def liftIO (t : Except String α ) : IO α :=
+
+def liftIO (t : ExceptT String Id α) : IO α := do
   match t with
   | .ok r => EStateM.Result.ok r
   | .error s => EStateM.Result.error s
 
+instance myFunkyName : MonadLift (ExceptT String Id) IO where
+  monadLift := liftIO
+
+-- set_option trace.Meta.synthInstance true in
 def main (args: List String): IO Unit := do
   try
-    let ret ← liftIO (divideRefactored 5 0 args 10)
+    let ret ← divideRefactored 5 0 |>.run args |>.run 10
     IO.println (toString ret)
   catch e =>
     IO.println e
