SimpleMonads/readme.md
@@ -24,20 +24,20 @@ terminal IO, networking, logging, exception handling, and reading or writing som
 settings, or state.  Monads can solve this problem, and they can be used for other useful things
 like metaprogramming.
 
-More generally monads are useful when you want to introduce a new concept to your programs
-without messing up the clarity, composability and maintainability of your pure functions.
+More generally monads are useful when you want to introduce a new concept to your programs without
+messing up the clarity, composability and maintainability of your pure functions.
 
 For example, suppose your Lean program must not allow divide by zero because that might cause
 your variables to get tainted with `Float.inf` and let's pretend that for your particular application
 that would be a huge problem (there are many real world applications where this is the case).
 
-But you don't want to change the `Float` to something else that means `Float` but never `Float.inf`
-because that would then mean you lose the nice benefits of the system provided `Float` type.
-So how can you get the compiler to ensure that `Float.inf` never happens in your program?
+But you don't want to stop using the `Float` because that would then mean you lose the nice benefits
+of the system provided `Float` type. So how can you get the compiler to ensure that `Float.inf`
+never happens in your program?
 
-There is a `Monad` defined in lean that adds exception handling behavior as an add on feature
-and the way you do it is to add to your return type information about the exception handling
-behavior your function might have:
+There is a `Monad` defined in lean that adds exception handling behavior as an add on feature and
+the way you do it is to add to your return type information about the exception handling behavior
+your function might have:
 
 ```lean
 def divide (x: Float ) (y: Float): ExceptT String Id Float :=
@@ -60,14 +60,12 @@ of the `ExceptT` monad to convert the floating point return value `x / y` into t
 
 This return typing would get tedious if you had to include it everywhere that you call this
 function, however, Lean type inference can clean this up. For example, you can define a test
-function can calls the `divide` function with lots of values and you don't need to say anything here
-about the fact that it might throw an error, because that is inferred:
+function can calls the `divide` function and you don't need to say anything here about the fact that
+it might throw an error, because that is inferred:
 
 ```lean
 def test :=
-  for x in [1:10] do
-    for y in [0:10] do
-      discard (divide x.toFloat y.toFloat)
+  divide 5 0
 ```
 
 The Lean compiler propagates the type information for you:
@@ -93,11 +91,12 @@ def testCatch := do
     return s!"Caught exception: {e}"
 ```
 
-Note that the type inferred by Lean for this function is `ExceptT String Id String` so the `ExceptT
-String Id Float` return type from the divide has been transformed. The ok type changed from `Float`
-to `String`. This is called "monad transformation" and is what the T stands for in `ExceptT`.  The
-secret to Lean is how easily it does monad transformation for you in most cases.  Notice here you
-didn't have to do any extra work for the compiler to figure out the transform you were trying to do.
+Note that the type inferred by Lean for this function is `ExceptT String Id String` so the
+`ExceptT String Id Float` return type from the divide has been transformed.
+The ok type changed from `Float` to `String`. This is called "monad transformation" and is
+what the T stands for in `ExceptT`.  The secret to Lean is how easily it does monad transformation
+for you in most cases.  Notice here you didn't have to do any extra work for the compiler to figure
+out the transform you were trying to do.
 
 You can now see the try/catch working in this eval:
 
@@ -118,15 +117,15 @@ So what really just happened under the covers? Exceptions start with this induct
 
 ```lean
 inductive Except (ε : Type u) (α : Type v) where
-  | error : ε → Except ε α -- A failure value of type `ε`
-  | ok    : α → Except ε α -- A success value of type `α`
+  | error : ε → Except ε α
+  | ok    : α → Except ε α
 ```
 
-It can represent an error case where the error is any type `ε` or an ok case where the ok value is
-any type `α`.  So the type `Except String Float` represents an exception that has a string in the
-error case or a floating point value in the ok case.
+Notice this is very generic it can represent an error case where the error is any type `ε` or an ok
+case where the ok value is any type `α`.  So the type `Except String Float` represents an Except
+type that has a string in the error case or a floating point value in the ok case.
 
-This Except type is then turned into a Monad by declaring this Monad type instance:
+This Except type is then turned into a `Monad` by declaring this Monad type instance:
 
 ```lean
 instance : Monad (Except ε) where
@@ -147,16 +146,33 @@ the type `Except ε α` to create a new return type, whatever type is defined by
 to use here.  The `T` in `ExceptT` is short for "transformer", so `ExceptT` is a monad based type
 transformer.
 
+| side note |
+| ----- |
+| Now remember that in Lean, any function `f (x) (y) (z)` can be turned into compositional subfunctions, so `f x y` is a function that returns a function that takes a `z` and `f x` is a function that returns a function that takes `y z` and so on.  This is a type of currying.  This means: |
+
+- `ExceptT String` is a monad transformer.
+- `ExceptT String Id` is a monad.
+- `ExceptT String Id Float` is a monadic action in the monad `ExceptT String Id` which produces a Float
+when you call the `run` method on that action.
+
+Yes `ExceptT` also provides a `run` method as follows:
+```lean
+def ExceptT.run {ε : Type u} {m : Type u → Type v} {α : Type u} (x : ExceptT ε m α) : m (Except ε α) := x
+```
+
+Now the `#eval` command can implicitly call `run` for you in some cases, so when we did `#eval test`
+we were really doing this:
+
+```lean
+#eval test.run
+```
+
 Now the `divide` function is using the `Id` monad which is the identity transform so the return type
 in this case will be unchanged `Except String Float`.  This `Id` monad might seem a bit weird right
-now, but later we will see how we can replace that with something more useful.
+now, but it is a placeholder that will allow us to chain monads, which we will do later.
 
-So the `divide` function can return an Exception object containing an error of type `String` or a ok
+So the `divide` function can return an Exception object containing an error of type `String` or an ok
 result of type Float - which is exactly what we wanted.
-
-But notice that our `test` function discards the result of the `divide` since it is just a test, and
-therefore lean has figured out that the `test` function then has a different `ok` type, namely
-`PUnit`, which is the type meaning no value is returned.
 
 The divide function also used this `pure` function which is defined as :
 
@@ -168,7 +184,7 @@ def pure {ε : Type u} (a : α) : Except ε α :=
 
 So in the case of `Except String Float` the implicit error type `ε` is `String` and the pure value
 is a `Float` and the `Except.pure` implementation then simply uses the `Except.ok` constructor
-passing the pure value to be wrapped in an Except object.  So `pure (x / y)` converts the pure value
+passing the pure value to be wrapped in an `Except` object.  So `pure (x / y)` converts the pure value
 `x / y` into something that matches the return type `Except String Float`.
 
 All this is built on the `Monad` type class which is defined as follows:
@@ -187,8 +203,8 @@ Remember that type classes in Lean allow the compiler to do type inference using
 instances.  So the instance `Monad (Except ε)` allows the compiler to invoke `Except.pure` when we
 call the `pure` method, and `Except.bind` if we call `bind` and so on.
 
-Notice the `instance : Monad (Except ε) ` doesn't define the ok type `(α : Type v)`. If you `#check
-(Except String)` you will find you get a function that operates on types.
+Notice the `instance : Monad (Except ε)` doesn't define the ok type `(α : Type v)`. If you
+`#check (Except String)` you will find you get a function that operates on types, in other words a monad:
 ```lean
 Except String : Type u_1 → Type (max 0 u_1)
 ```
@@ -216,25 +232,57 @@ namespace Except
   | Except.ok v      => f v
 ```
 
-So this bind function can be used to transform the type `Except String Float` to `Except String
-String`.  First we need a function that takes `Float → Except String String` and it then unwraps the
+So this bind function can be used to transform the type `Except String Float` to `Except String String`.
+First we need a function that takes `Float → Except String String` and it then unwraps the
 given `Except String Float` into its `error` and `ok` cases, passing the error through unchanged as
-`Except.error err` but using the function to transform the `ok` variable `v` into a string by
+`Except.error err` and using the function `f` to transform the `ok` variable `v` into a string by
 applying `f v` which returns a new type `Except String String`.
 
 This transformation happened automatically in the `testCatch` function earlier because we used the
 `do` notation which is a powerful tool that can chain monad actions finding and applying the right
 bind operations automatically when needed. In the `testCatch` function the following line of code
-shows how this works:
+shows this in action:
 
 ```lean
     return toString r -- ExceptT String Id String
 ```
-Here the `toString` function was composed into something that contructs an `Except.ok string`
+Here the `toString` function was composed into something that contructs an `Except.ok String`
 result.  So this monad type inference and composition of binding operations is pretty powerful.
 
-You can also use `bind` manually if you want to control how it works which we'll see below.
+Now you might be wondering why `testCatch` doesn't have return type `String`? Lean does this as a
+convenience since you could have a rethrow in or after the catch block. If you really want to stop
+the `ExceptT` type from bubbling up you can do this:
 
+```lean
+def testUnwrap : String := Id.run do
+    let r := divide 8 0 -- r is type ExceptT String Id Float = Except String Float
+    match r with
+    | .ok a => toString a -- 'a' is type Float
+    | .error e => s!"Caught exception: {e}"
+
+#check testUnwrap -- String
+#eval testUnwrap -- "Caught exception: can't divide by zero"
+```
+
+Alternatively you could solve this using coercions, although that is not always recommended.
+
+```lean
+instance : Coe (ExceptT α Id α) α where
+  coe a := match a with
+    | .ok v => v
+    | .error v => v
+
+def testCoerce : String :=
+  let act : ExceptT String Id String := do
+    let r ← divide 8 0
+    return r.toString
+  act
+
+#check testCoerce -- String
+#eval testCoerce  -- "can't divide by zero"
+```
+
+You can also use `bind` manually if you want to control how it works which we'll see below.
 
 ## Monad Composition
 
@@ -251,9 +299,14 @@ light weight, and easier to consume programmatically.  So let's create a counter
 incremented every time divide succeeds and pass that "logging state" into our program so you can
 then also read that state when the program is finished.
 
-There is a monad already defined for this kind of stateful side effect, it is called `MonadStateOf`:
+There is a monad already defined for this kind of stateful side effect, it is called `StateT`:
 
 ```lean
+def StateT (σ : Type u) (m : Type u → Type v) (α : Type u) : Type (max u v) :=
+  σ → m (α × σ)
+```
+which has some additional functions available through `MonadStateOf`:
+```
 instance [Monad m] : MonadStateOf σ (StateT σ m) where
   get       := StateT.get
   set       := StateT.set
@@ -271,11 +324,47 @@ def divideLog (x: Float ) (y: Float): StateT Nat Id Float :=
   if y == 0 then do
     return 0
   else do
-    (modify) fun s => s + 1
+    modify fun s => s + 1
     return x / y
 ```
 
-`modify` is a helper that makes it easier to use modifyGet.
+But how does adding a return type of `StateT` allow stateful "inputs" to be passed to the divideIt
+function?  How can a return type add an input? You can use "currying" again check the reduced type:
+
+```lean
+#check divideLog              -- Float → Float → StateT Nat Id Float
+#reduce StateT Nat Id Float   -- Nat → Float × Nat
+```
+
+So effectively StateT has changed our function into:
+
+```
+Float → Float → Nat → Float × Nat
+```
+
+So `StateT` has turned the return type into a function that takes a natural number as input and
+returns the updated state in the pair `Float × Nat`. So it has essentially then added an input
+parameter to our `divideLog` function.  This parameter can be accessed by the `StateT`
+interface `get`, and `modifyGet`. `modify` is a helper that makes it easier to use `modifyGet`.
+
+The following 3 ways of calling this function are equivalent:
+```lean
+#eval divideLog 8 4 0         -- (2.000000, 1)
+#eval (divideLog 8 4).run 0   -- (2.000000, 1)
+#eval divideLog 8 4 |>.run 0  -- (2.000000, 1)
+```
+
+The first way of simply tacking on the state argument is not recommended because it makes your
+code hard to maintain if the divideLog parameters change or the StateT monad is changed and so on.
+it is better to use the `run` method explicitly which you can do using parentheses, but if you
+have lots of monads in your chain the right associative operator '|>' is more convenient as it
+drops the need for parentheses.
+
+An added benefit of calling `run` explicitly is that the Lean type checker will always ensure for
+you that the result of `divideLog 8 4` is a type that has some `run` method and so on, if this is
+not the case it will highlight the right section of your code instead of giving a confusing big
+error on your entire application that contains some weird monad stack mess. So this is the
+recommended pattern.
 
 You can call this function in a test function, passing in the state on each call, and storing the
 updates in a mutable state variable and with the nested for loops this will divide by zero exactly
@@ -286,7 +375,7 @@ def testDivideLog := do
   let mut state := 0
   for x in [0:10] do
     for y in [0:10] do
-      let r ← (divideLog x.toFloat y.toFloat) state
+      let r ← (divideLog x.toFloat y.toFloat) |>.run state
       state := r.2
   state
 
@@ -294,16 +383,26 @@ def testDivideLog := do
 ```
 
 Great, a completely different example of adding an orthogonal dimension to our code (logging).  But
-now what if we want both logging and exception handling? Well you can chain StateT, and ExceptT
-because remember they take a monad as input.  We were passing `Id` before, but now we can pass the
-monad `ExceptT String Id` instead resulting in the return type `StateT Nat (ExceptT String Id)
-Float`! Phew, that's a mouth full.  Lean allows very sophisticated type construction.
+now what if we want both logging and exception handling? Well you can chain `StateT`, and `ExceptT`
+-- this is why the `*T` monad transformers take a monad as input.  We were passing `Id` before, but
+now we can pass the monad `ExceptT String Id` instead resulting in the return type
+`StateT Nat (ExceptT String Id) Float`! Phew, that's a mouth full.  Lean allows very sophisticated type
+construction.
 
 So this means `StateT` will transform `Except String Float` into some new return type, in this case
-it will become `Except String (Float × Nat)` because we need the modified state to be returned as
-well as the division result, so they are returned as a pair.
+it will become `Nat → Except String (Float × Nat)` because we need the to be able to pass in the state
+and get back the modified state, so it returns the division result, and the updated state as a tuple.
 
-Here's the combined monadic function:
+You can now use `bind` manually to chain the 2 monadic functions, in this case (`modify` from StateT
+and `pure` from `ExceptT`) and the `bind` function on StateT is defined as:
+
+```lean
+@[inline] protected def bind (x : StateT σ m α) (f : α → StateT σ m β) : StateT σ m β :=
+  fun s => do let (a, s) ← x s; f a s
+```
+
+So it returns the pair `(a, s)` which means in this case `β` is inferred to be the
+type `Float × Nat`.  Here's the combined monadic function using a manual bind:
 
 ```lean
 def divideIt (x:Float) (y:Float) : StateT Nat (ExceptT String Id) Float :=
@@ -315,34 +414,11 @@ def divideIt (x:Float) (y:Float) : StateT Nat (ExceptT String Id) Float :=
 #check divideIt -- Float → Float → StateT Nat (ExceptT String Id) Float
 ```
 
-But how does adding a return type of `StateT` allow stateful "inputs" to be passed to the divideIt
-function?  How can a return type add an input? You can use "currying", check the reduced type:
-
 ```lean
-#reduce StateT Nat (ExceptT String Id) Float -- Nat → Except String (Float × Nat)
+#eval divideIt 5 2 |>.run 0 -- Except.ok (5.000000, 1)
 ```
 
-So StateT has turned the return type into a function that takes a natural number as input and
-returns the natural number in the pair `Float × Nat`. So it has essentially then added an input
-parameter to our function, but it doesn't have a name, and can only be accessed by the StateT
-interface `get`, and `modifyGet`.
-
-You can now use `bind` manually to chain the 2 monadic functions, in this case (`modify` from StateT
-and `pure` from `ExceptT`) and the `bind` function on StateT is defined as:
-
-```lean
-@[inline] protected def bind (x : StateT σ m α) (f : α → StateT σ m β) : StateT σ m β :=
-  fun s => do let (a, s) ← x s; f a s
-```
-
-So it returns the pair `(a, s)` which means in this case `β` is inferred to be the
-type `Float × Nat`:
-
-```lean
-#eval divideIt 5 1 0 -- Except.ok (5.000000, 1)
-```
-
-The 3rd parameter passed here is the initial value of the `StateT Nat` being passed in. The function
+The `run` parameter passed here is the initial value of the `StateT Nat` being passed in. The function
 incremented this state and returned it as the second member of the pair `(5.000000, 1)`.
 
 You can test this new composite `divideIt` function in a very similar way to `testDivideLog` and you
@@ -354,7 +430,7 @@ def testIt := do
   for x in [0:10] do
     for y in [0:10] do
       try
-        let r ← divideIt x.toFloat y.toFloat log
+        let r ← divideIt x.toFloat y.toFloat |>.run log
         log := r.2
       catch _  =>
         pure ()
@@ -364,11 +440,11 @@ def testIt := do
 ```
 
 Notice here the extracted value in `r` is the pair `Float × Nat` so `r.2` then is the updated
-`state`, or the count of times we did a successful divide and we get the same result, 90 good
-divides.
+`state` which we want to keep around so we get the running tally of the number of times we did a
+successful divide and we get the same result: 90 good divides.
 
-Ok, now to bring it all together, you don't need to use `bind` manually like this because the `do
-Notation` can chain monadic actions using bind automatically, so you can rewrite the divideIt
+Ok, now to bring it all together, you don't need to use `bind` manually like this because the
+`do` notation can chain monadic actions using bind automatically, so you can rewrite the divideIt
 function as:
 
 ```lean
@@ -376,68 +452,77 @@ def divideDo (x:Float) (y:Float) : (StateT Nat (ExceptT String Id)) Float := do
   if y == 0 then
     throw "can't divide by zero"
   else
-    (modify fun s => s + 1)
+    modify fun s => s + 1
     pure (x / y)
 ```
 
 So here the do Notation DSL generated the code `bind (modify fun s => s + 1) (fun _ => pure (x / y))`
 for you.  Pretty neat.  Note that we used the do notation in `divideLog` to do some chaining also.
 
-So an imperative program can be modelled in functional language as a chain of monadic actions :-)
+So an imperative program can be modelled in a functional language as a chain of monadic actions
+and this is a major innovation in the Lean language.
 
 ## Add one more for fun!
 
 `ReaderT` is like `StateT` but it is read only, so it is ideal for "context" or "global state". We
 can use it to pass around our command line arguments so different parts of our program can behave
-differently as a result of those arguments.  Let's first see the manual binding so you get a better
-idea of how they compose:
+differently as a result of those arguments.  `ReaderT` provides the additional function `read`
+to access that read only context.
+
+Let's first see the manual binding so you get a better idea of how they compose:
 
 ```lean
-def divide (x:Float) (y:Float) : ReaderT (List String) (StateT Nat (ExceptT String Id)) Float :=
-  if y == 0 then
-    throw "can't divide by zero"
-  else
-    bind (modify fun s => s + 1) fun _ =>
-      bind (get) fun s =>
-        bind (read) fun args =>
-          if (s > 10 && args.contains "--limit") then
-            throw "too many tries"
-          else
-            pure (x / y)
+def divideWithArgs (x:Float) (y:Float) : ReaderT (List String) (StateT Nat (ExceptT String Id)) Float :=
+  bind (modify fun s => s + 1) fun _ =>
+    bind (get) fun s =>
+      bind (read) fun args =>
+        if (s > 10 && args.contains "--limit") then
+          throw "too many divides"
+        else if y == 0 then
+          throw "can't divide by zero"
+        else
+          pure (x / y)
 
 /-
 List String → Nat → Except String (Float × Nat)
 -/
 #reduce ReaderT (List String) (StateT Nat (ExceptT String Id)) Float
 
-#eval divideWithArgs 5 2 [] 0 -- Except.ok (2.500000, 1)
-#eval divideWithArgs 5 0 [] 0 -- Except.error "can't divide by zero"
-#eval divideWithArgs 5 2 ["--limit"] 10 -- Except.error "too many divides"
+#eval divideWithArgs 5 2 |>.run [] |>.run 0 -- Except.ok (2.500000, 1)
+#eval divideWithArgs 5 0 |>.run [] |>.run 0 -- Except.error "can't divide by zero"
+#eval divideWithArgs 5 2 |>.run ["--limit"] |>.run 10 -- Except.error "too many divides"
 ```
 
-And of course `do` Notation cleans this up very nicely:
+Notice that because we have added 2 monads now, `ReaderT` and `StateT` we want to see 2 `run` method
+calls.
+
+Fortunately, tThe `do` Notation cleans this up very nicely:
 
 ```lean
 def divideWithArgsDo (x:Float) (y:Float) : ReaderT (List String) (StateT Nat (ExceptT String Id)) Float := do
-  if y == 0 then
+  modify fun s => s + 1
+  let s ← get
+  let args ← read
+  if (s > 10 && args.contains "--limit") then
+    throw "too many divides"
+  else if y == 0 then
     throw "can't divide by zero"
   else
-    modify fun s => s + 1
-    let s ← get
-    let args ← read
-    if (s > 10 && args.contains "--limit") then
-      throw "too many divides"
-    else
-      pure (x / y)
+    pure (x / y)
 
-#eval divideWithArgsDo 5 2 [] 0 -- Except.ok (2.500000, 1)
-#eval divideWithArgsDo 5 0 [] 0 -- Except.error "can't divide by zero"
-#eval divideWithArgsDo 5 2 ["--limit"] 10 -- Except.error "too many divides"
+#eval divideWithArgsDo 5 2 |>.run [] |>.run 0 -- Except.ok (2.500000, 1)
+#eval divideWithArgsDo 5 0 |>.run [] |>.run 0 -- Except.error "can't divide by zero"
+#eval divideWithArgsDo 5 2 |>.run["--limit"] |>.run 10 -- Except.error "too many divides"
 ```
 
-Oooh, isn't that loverly.
+Oooh, isn't that loverly.  You can even prove that these functions are equivalent:
 
-## Lifting
+```lean
+example : divideWithArgs x y = divideWithArgsDo x y := by
+  simp[divideWithArgs, divideWithArgsDo]    -- Goals accomplished 🎉
+```
+
+## Monad Lifting
 
 An important part of any program is functional decomposition, breaking large functions up into
 smaller ones. When you do that you don't always want the smaller functions to have the big complex
@@ -464,40 +549,47 @@ def divideRefactored (x:Float) (y:Float) : ReaderT (List String) (StateT Nat (Ex
   else
     divide x y
 
-#eval divideRefactored 5 0 [] 0 -- Except.error "can't divide by zero"
+#eval divideRefactored 5 2 |>.run [] |>.run 0 -- Except.ok (2.500000, 1)
+#eval divideRefactored 5 0 |>.run [] |>.run 0 -- Except.error "can't divide by zero"
+#eval divideRefactored 5 2 |>.run ["--limit"] |>.run 10 -- Except.error "too many divides"
 ```
 
 Very cool - but some magic happened here. The smaller `divide` function has a different return type
-`ExceptT String Id Float` yet you returned it's value no problem and the compiler turned it into
-`ReaderT (List String) (StateT Nat (ExceptT String Id)) Float` for you somehow.
+`ExceptT String Id Float` yet you returned it's value no problem and the compiler turned that into
+`ReaderT (List String) (StateT Nat (ExceptT String Id)) Float` for you, somehow.
 
-This is called "monad lifting" and is another secret sauce that Lean provides that make monads super
-easy to use.  You could imagine manual monad lifting would be very tedious indeed. You can see this
-in action with the following test:
+This is called "monad lifting" and is another secret sauce that Lean provides in order to make
+monads super easy to use.  You could imagine manual monad lifting would be very tedious indeed. You
+can see this in action with the following test:
 
 ```lean
 def lift1 (x : ExceptT String Id Float) : (StateT Nat (ExceptT String Id)) Float :=
   x
 
-#eval lift1 (divide 5 1) 3 -- Except.ok (5.000000, 3)
+#eval lift1 (divide 5 1) |>.run 3 -- Except.ok (5.000000, 3)
 ```
 
-You can see this is lifted because the `Execpt.ok` value is a pair.
-Now we need a second lift to ReaderT:
+You can see this is lifted to `StateT` because we were able to then `.run` that with initial state `3`
+and the StateT monad converted that into the pair `(5.000000, 3)`.  `lift1` didn't modify the state
+so it came back to us unmodified.  Now we need a second lift to ReaderT:
 
 ```lean
 def lift2 (x : StateT Nat (ExceptT String Id) Float) : ReaderT (List String) (StateT Nat (ExceptT String Id)) Float :=
   x
 
-#eval lift2 (lift1 (divide 5 1)) [] 0 -- Except.ok (5.000000, 0)
+#eval lift2 (lift1 (divide 5 1)) |>.run ["discarded", "state"] |>.run 4 -- Except.ok (5.000000, 4)
 ```
 
-So you can see how the lifts compose nicely, we can pass in the ReaderT args, and the initial state, and
-we get back the divide result and the returned state.
+So you can see how the lifts compose nicely, we can pass in the `ReaderT` args, and the initial
+state, and we get back the divide result and the returned state. In this case `lift2` does nothing
+with the `ReaderT` args so they are discarded.
 
-So what Lean did for you here is a transitive closer of lifting operations. Let's see how that
-works.  If you `#print` lift1 you will see it is implemented as `fun x => liftM x` and `liftM` is an
-abbreviation for `monadLift` from `MonadLiftT`.
+So what Lean did for you in `divideRefactored` is a transitive closure of monad lifting operations!
+
+## Lifting Deep Dive
+
+Let's see how that works.  If you `#print lift1` you will see it is implemented as `fun x => liftM x` and
+`liftM` is an abbreviation for `monadLift` from `MonadLiftT`.
 
 ```lean
 class MonadLiftT (m : Type u → Type v) (n : Type u → Type w) where
@@ -506,14 +598,14 @@ class MonadLiftT (m : Type u → Type v) (n : Type u → Type w) where
 ```
 
 The `T` in `MonadLiftT` stands for "transitive" it is able to transitively lift monadic computations
-using `MonadLift` which is a function for for lifting a computation from an inner `Monad` to an
+using `MonadLift` which is a function for lifting a computation from an inner `Monad` to an
 outer `Monad`.
 
 So now we can check all the `MonadLift` instances defined in Lean, and in our case we will be using:
 
 ```lean
 instance : MonadLift m (StateT σ m)  -- to lift to StateT
-instance  : MonadLift m (ReaderT ρ m) -- to lift to ReaderT
+instance : MonadLift m (ReaderT ρ m) -- to lift to ReaderT
 ```
 
 These instances override the `lift` function for these types, showing the compiler how to generate
@@ -524,12 +616,12 @@ that code.  Let's see how that works for StateT:
   fun s => do let a ← t; pure (a, s)
 ```
 
-So given some implicit type `α` and a monad `m` that acts on `α` it is able to generate the return
-type `StateT σ m α` by returning a function that takes some state `s` from which it can then create
-the pair (a, s) where `a` is the result of applying the monad `m α`.  And this is what we saw, the
-state `0` passed in resulted in a pair coming back out as `(5.000000, 0)`.  It is not inventing the
-state, it is lifting that state so it is an input and an output resulting in a valid `StateT Nat
-(ExceptT String Id)`.
+So this is very generic, given some implicit type `α` and a monad `m` that acts on `α` it is able to
+generate the return type `StateT σ m α` by returning a function that takes some state `s` from which
+it can then create the pair `(a, s)` where `a` is the result of applying the monad `m α`.  And this
+is what we saw, the state `3` passed in resulted in a pair coming back out as `(5.000000, 3)`.  It
+is not inventing the state, it is lifting that state so it is an input and an output resulting in a
+valid `StateT Nat (ExceptT String Id)`.
 
 Similarly, for `ReaderT` we find:
 
@@ -538,62 +630,86 @@ instance  : MonadLift m (ReaderT ρ m) where
   monadLift x := fun _ => x
 ```
 This one is a bit simpler, remember `ReaderT` is about passing in some read-only state, but to lift
-something that does not know about `ReaderT` then it obviously doesn't care about this read only
-state, so we can throw it away using the underscore `_` and simply return the type being lifted,
-which is what we saw with this eval:
+from something that does not know about `ReaderT` then the thing we are calling obviously doesn't
+care about this read only state, so we can throw it away using the underscore `_` and simply call
+the inner function, which is what we saw with this eval:
 
 ```lean
-#eval lift2 (lift1 (divide 5 1)) ["discarded", "state"] 0 -- Except.ok (5.000000, 0)
+#eval lift2 (lift1 (divide 5 1)) |>.run ["discarded", "state"] |>.run 4 -- Except.ok (5.000000, 4)
 ```
 
-The ReaderT state here is `["discarded", "state"]` and it is thrown away when calling lift1 because
-`lift1` doesn't know about ReaderT.
+The ReaderT state here is `["discarded", "state"]` and it is thrown away when calling `lift1`
+because `lift1` doesn't know (or care) about `ReaderT`.
 
 So looking at `divideRefactored` again, you get an appreciation for what is going on under the
 covers to make that monadic code nice and composable, both on the way in with monads like `ReaderT`
 and `StateT` adding additional input parameters, and on the way out with automatic transitive monad
 lifting. Lift happens very often in Lean.
 
-## Testing
+## Add your own Custom Lifting
 
-You can now build the app with `lake build` and try out your main function:
+You can now build the app with `lake build` and try out this main function:
 
 ```lean
 def main (args: List String): IO Unit := do
   try
-    let ret ← liftIO  (divideRefactored 5 0 args 10)
+    let ret ← divideRefactored 5 0 |>.run args |>.run 10
     IO.println (toString ret)
   catch e =>
     IO.println e
 ```
 
-This function does not compile without the `liftIO` conversion here because `divideRefactored`
-returns our big `ReaderT (List String) (StateT Nat (ExceptT String Id)) Float` but that cannot
-be automatically transformed into the `main` return type of `IO Unit` so `liftIO` is designed
-to do that conversion:
+This function would not normally compile saying:
+```
+typeclass instance problem is stuck, it is often due to metavariables
+```
+and you can see this error if you add this line before the `main` function:
+```
+set_option autoLift false
+```
+
+`divideRefactored` returns the big `ReaderT (List String) (StateT Nat (ExceptT String Id)) Float`
+and the problem is that cannot be automatically transformed into the `main` return type of `IO Unit`
+unless we give it some help.
+
+The following custom `MonadLift` solves this problem:
 
 ```lean
-def liftIO (t : Except String α ) : IO α :=
+def liftIO (t : ExceptT String Id α) : IO α := do
   match t with
   | .ok r => EStateM.Result.ok r
   | .error s => EStateM.Result.error s
+
+instance : MonadLift (ExceptT String Id) IO where
+  monadLift := liftIO
 ```
 
-If you dive into `IO` you will see it is an abbreviation for `EIO Error` and `EIO` is a function
-that transforms into `EStateM Error IO.RealWorld` and `Error` is from the `IO` namespace and is an
-inductive type with lots of possible errors.  `EStateM` creates a `Result` object with `ok` and
-`error` values, very similar to `Except`, but with one more parameter.
+This instance makes it possible to lift the result of type `ExceptT String Id` into the type
+required by main which is `IO Unit`. Fortunately this lift is relatively easy because IO is just an
+alias for the `EStateM.Result` which is very similar to the `Except` object in that it also has an
+`ok` or `error` state. The difference is `Result` has one more data member, which is a return code.
 
-`lake build` will create a binary named `simpleMonads` which  you can run from the command line and
+If we have an instance `MonadLiftT m n` that means there is a way to turn a computation that happens
+inside of `m` into one that happens inside of `n` and (this is the key part) usually *without* the
+instance itself creating any additional data that feeds into the computation. This means you can in
+principle declare lifting instances from any monad to any other monad, it does not, however, mean that
+you should do this in all cases.  You can get a report from Lean of how all this was done by
+uncommenting the line `set_option trace.Meta.synthInstance true in` before main and moving the
+cursor to the end of the first line after `do` and you will see a nice detailed report.
+
+Now `lake build` will create a binary named `simpleMonads` which  you can run from the command line and
 you can pass command line parameters as follows:
 
 ```
-simpleMonads
+> simpleMonads
 can't divide by zero
 
-simpleMonads --limit
+> simpleMonads --limit
 too many divides
 ```
 
 So we were able to influence the behavior of our program by passing some command line arguments and
-some logging state, and we added some exception handling all in a purely functional way using monads.
+some logging state, and we added some exception handling and we did it all in a purely functional
+way using monads.  Then we also showed how monad lifing makes functional decomposition nice and
+manageable.
+
